Removed external state and ExtGet

src/theory/bir-support/bir_exp_congruencesScript.sml
@@ -25,26 +25,29 @@ val _ = new_theory "bir_exp_congruences";
    simplification. *)
 
 Definition bir_eval_exp_EQUIV_def:
-  bir_eval_exp_EQUIV e1 e2 = !env ext_st.
-    bir_eval_exp e1 env ext_st = bir_eval_exp e2 env ext_st
+  bir_eval_exp_EQUIV e1 e2 = !env.
+    bir_eval_exp e1 env = bir_eval_exp e2 env
 End
 
-val bir_eval_exp_EQUIV_IS_EQUIV = store_thm ("bir_eval_exp_EQUIV_IS_EQUIV",
-  ``(!e. bir_eval_exp_EQUIV e e) /\
+Theorem bir_eval_exp_EQUIV_IS_EQUIV:
+  (!e. bir_eval_exp_EQUIV e e) /\
     (!e1 e2. bir_eval_exp_EQUIV e1 e2 <=> bir_eval_exp_EQUIV e2 e1) /\
     (!e1 e2 e3. bir_eval_exp_EQUIV e1 e2 ==> bir_eval_exp_EQUIV e2 e3 ==>
-                bir_eval_exp_EQUIV e1 e3)``,
-METIS_TAC[bir_eval_exp_EQUIV_def]);
+                bir_eval_exp_EQUIV e1 e3)
+Proof
+METIS_TAC[bir_eval_exp_EQUIV_def]
+QED
 
 
 (* It is a congruence, it works with substitution *)
 
-val bir_eval_exp_EQUIV_IS_CONG_SUBST = store_thm ("bir_eval_exp_EQUIV_IS_CONG_SUBST",
-``!v ve ve' e. bir_eval_exp_EQUIV ve ve' ==>
-               bir_eval_exp_EQUIV (bir_exp_subst1 v ve e) (bir_exp_subst1 v ve' e)``,
-
+Theorem bir_eval_exp_EQUIV_IS_CONG_SUBST:
+  !v ve ve' e. bir_eval_exp_EQUIV ve ve' ==>
+               bir_eval_exp_EQUIV (bir_exp_subst1 v ve e) (bir_exp_subst1 v ve' e)
+Proof
 SIMP_TAC std_ss [bir_eval_exp_EQUIV_def] >>
-METIS_TAC[bir_exp_subst1_EVAL_EQ_GEN]);
+METIS_TAC[bir_exp_subst1_EVAL_EQ_GEN]
+QED
 
 
 (****************************)
@@ -62,12 +65,10 @@ Definition bir_exp_CONG_def:
   bir_exp_CONG e1 e2 <=>
     type_of_bir_exp e1 = type_of_bir_exp e2 /\
     bir_vars_of_exp e2 = bir_vars_of_exp e1 /\
-    bir_exts_of_exp e1 = bir_exts_of_exp e2 /\
-    !env ty ext_st.
-      bir_env_vars_are_initialised env (bir_vars_of_exp e1) /\
-      type_of_bir_exp e1 = SOME ty /\
-      bir_ext_env_exts_are_valid ext_st (bir_exts_of_exp e1) ==>
-      bir_eval_exp e1 env ext_st = bir_eval_exp e2 env ext_st
+    !env ty.
+      bir_env_vars_are_initialised env (bir_vars_of_exp e1) ==>
+      type_of_bir_exp e1 = SOME ty ==>
+      bir_eval_exp e1 env = bir_eval_exp e2 env
 End
 
 Theorem bir_exp_CONG_REFL:
@@ -98,51 +99,6 @@ Proof
   >> fs[bir_exp_CONG_def]
 QED
 
-Theorem bir_exts_of_exp_bir_exp_subst1:
-  !e ve ve' v.
-    bir_vars_of_exp ve = bir_vars_of_exp ve'
-    /\ bir_exts_of_exp ve = bir_exts_of_exp ve' ==>
-  bir_exts_of_exp (bir_exp_subst1 v ve e) =
-  bir_exts_of_exp (bir_exp_subst1 v ve' e)
-Proof
-  Induct
-  >> fs[bir_exp_subst1_REWRS]
-  >> rw[]
-  >> fs[bir_exts_of_exp_def,bir_vars_of_exp_def]
-  >> qmatch_goalsub_rename_tac `bir_exp_subst1 v _ _`
-  >> rpt $ first_x_assum $ drule_all_then $ qspec_then `v` assume_tac
-  >> fs[]
-QED
-
-Theorem bir_ext_env_exts_are_valid_bir_exp_subst1:
-  !e ext_st v ve.
-  bir_ext_env_exts_are_valid ext_st (bir_exts_of_exp (bir_exp_subst1 v ve e))
-  ==> bir_ext_env_exts_are_valid ext_st (bir_exts_of_exp e)
-Proof
-  Induct
-  >> fs[bir_exts_of_exp_def,bir_env_oldTheory.bir_ext_env_exts_are_valid_EMPTY,bir_exp_subst1_REWRS]
-  >> asm_rewrite_tac[]
-  >> rpt strip_tac
-  >> fs[bir_env_oldTheory.bir_ext_env_exts_are_valid_UNION]
-  >> rpt $ first_x_assum drule_all
-  >> fs[]
-QED
-
-Theorem bir_ext_env_exts_are_valid_bir_exp_subst1':
-  !e ext_st v ve.
-  v IN bir_vars_of_exp e
-  /\ bir_ext_env_exts_are_valid ext_st (bir_exts_of_exp (bir_exp_subst1 v ve e))
-  ==> bir_ext_env_exts_are_valid ext_st (bir_exts_of_exp ve)
-Proof
-  Induct
-  >> fs[bir_exts_of_exp_def,bir_env_oldTheory.bir_ext_env_exts_are_valid_EMPTY,bir_exp_subst1_REWRS,bir_vars_of_exp_def]
-  >> asm_rewrite_tac[]
-  >> rpt strip_tac
-  >> fs[bir_env_oldTheory.bir_ext_env_exts_are_valid_UNION]
-  >> rpt $ first_x_assum drule_all
-  >> fs[]
-QED
-
 Theorem bir_exp_CONG_IS_CONG_SUBST:
   !v ve ve' e.
     bir_exp_CONG ve ve' ==>
@@ -155,17 +111,15 @@ Proof
   ) >>
   STRIP_TAC >>
   fs[bir_exp_CONG_def, bir_exp_subst1_TYPE_EQ_GEN, bir_exp_subst1_USED_VARS,
-     bir_env_oldTheory.bir_env_vars_are_initialised_UNION, bir_exts_of_exp_bir_exp_subst1] >>
+     bir_env_oldTheory.bir_env_vars_are_initialised_UNION] >>
   REPEAT STRIP_TAC >>
   drule_all_then strip_assume_tac bir_exp_subst1_NO_TYPE_SOME >>
-  drule_all_then assume_tac bir_ext_env_exts_are_valid_bir_exp_subst1 >>
-  drule_all_then assume_tac bir_ext_env_exts_are_valid_bir_exp_subst1' >>
   irule bir_exp_subst1_EVAL_EQ_GEN >>
   first_x_assum irule >>
   gs[]
 QED
 
-(* For practical purposed more insteresting is however a form that can be used
+(* For practical purposes more interesting is however a form that can be used
    as congruence rules. *)
 
 Theorem bir_exp_CONG_BASIC_CONG_RULES:
@@ -188,8 +142,6 @@ Theorem bir_exp_CONG_BASIC_CONG_RULES:
       bir_exp_CONG et et' ==>
       bir_exp_CONG ef ef' ==>
       bir_exp_CONG (BExp_IfThenElse c et ef) (BExp_IfThenElse c' et' ef')) /\
-  (!ext ty.
-      bir_exp_CONG (BExp_ExtGet ext ty) (BExp_ExtGet ext ty)) /\
   (!mem_e mem_e' a_e a_e' en ty.
       bir_exp_CONG mem_e mem_e' ==>
       bir_exp_CONG a_e a_e' ==>
@@ -201,9 +153,9 @@ Theorem bir_exp_CONG_BASIC_CONG_RULES:
       bir_exp_CONG (BExp_Store mem_e a_e en v_e) (BExp_Store mem_e' a_e' en v_e'))
 Proof
   SIMP_TAC (std_ss++holBACore_ss) [bir_exp_CONG_def,
-    bir_env_oldTheory.bir_env_vars_are_initialised_UNION, type_of_bir_exp_def, bir_exts_of_exp_def] >>
+    bir_env_oldTheory.bir_env_vars_are_initialised_UNION, type_of_bir_exp_def] >>
   REPEAT STRIP_TAC >> ASM_SIMP_TAC std_ss [] >> (
-    metis_tac[bir_env_oldTheory.bir_ext_env_exts_are_valid_UNION]
+    metis_tac[]
   )
 QED
 
@@ -219,10 +171,9 @@ Proof
   REPEAT STRIP_TAC >>
   ASM_SIMP_TAC std_ss [bir_exp_CONG_def, bir_vars_of_exp_def,
     UNION_IDEMPOT, type_of_bir_exp_def, pairTheory.pair_case_thm,
-    bir_eval_exp_def, FUN_EQ_THM, bir_exts_of_exp_def] >>
+    bir_eval_exp_def, FUN_EQ_THM] >>
   REPEAT STRIP_TAC >>
-  qmatch_goalsub_rename_tac `_ = bir_eval_exp e env x` >>
-  Cases_on `bir_eval_exp e env x` >- (
+  Cases_on `bir_eval_exp e env` >- (
     FULL_SIMP_TAC (std_ss++holBACore_ss) [bir_eval_bin_exp_def]
   ) >>
   qmatch_goalsub_rename_tac `SOME x'` >>
@@ -241,17 +192,17 @@ Proof
 QED
 
 
-val bir_exp_CONG_simp_IDEMPOTENT_OR = store_thm ("bir_exp_CONG_simp_IDEMPOTENT_OR",
-   ``!e.
+Theorem bir_exp_CONG_simp_IDEMPOTENT_OR:
+  !e.
      (?ty. bir_type_is_Imm ty /\ (type_of_bir_exp e = SOME ty)) ==>
-     bir_exp_CONG (BExp_BinExp BIExp_Or e e) e``,
-
+     bir_exp_CONG (BExp_BinExp BIExp_Or e e) e
+Proof
 REPEAT STRIP_TAC >>
 ASM_SIMP_TAC std_ss [bir_exp_CONG_def, bir_vars_of_exp_def,
   UNION_IDEMPOT, type_of_bir_exp_def, pairTheory.pair_case_thm,
-  bir_eval_exp_def, bir_exts_of_exp_def] >>
+  bir_eval_exp_def] >>
 REPEAT STRIP_TAC >>
-Cases_on `bir_eval_exp e env ext_st` >- (
+Cases_on `bir_eval_exp e env` >- (
   FULL_SIMP_TAC (std_ss++holBACore_ss) [bir_eval_bin_exp_def]
 ) >>
 subgoal `ty = type_of_bir_val x` >- (
@@ -266,7 +217,7 @@ rename1 `bir_bin_exp _ v v = v` >>
 Cases_on `v` >> (
   SIMP_TAC (std_ss++holBACore_ss) [wordsTheory.WORD_OR_IDEM]
 )
-);
+QED
 
 
 
@@ -283,44 +234,37 @@ Definition bir_exp_CONG_WEAK_def:
   bir_exp_CONG_WEAK e1 e2 <=> 
     type_of_bir_exp e1 = type_of_bir_exp e2 /\
     bir_vars_of_exp e2 SUBSET bir_vars_of_exp e1 /\
-    bir_exts_of_exp e2 SUBSET bir_exts_of_exp e1 /\
-    !env ty ext_st.
-      bir_env_vars_are_initialised env (bir_vars_of_exp e1) /\
-      type_of_bir_exp e1 = SOME ty /\
-      bir_ext_env_exts_are_valid ext_st (bir_exts_of_exp e1) ==>
-      bir_eval_exp e1 env ext_st = bir_eval_exp e2 env ext_st
+    !env ty.
+      bir_env_vars_are_initialised env (bir_vars_of_exp e1) ==>
+      type_of_bir_exp e1 = SOME ty ==>
+      bir_eval_exp e1 env = bir_eval_exp e2 env
 End
 
-val bir_exp_CONG_WEAK_IS_WEAK = store_thm ("bir_exp_CONG_WEAK_IS_WEAK",
- ``!e1 e2. bir_exp_CONG e1 e2 ==> bir_exp_CONG_WEAK e1 e2``,
+Theorem bir_exp_CONG_WEAK_IS_WEAK:
+  !e1 e2. bir_exp_CONG e1 e2 ==> bir_exp_CONG_WEAK e1 e2
+Proof
 SIMP_TAC std_ss [bir_exp_CONG_def, bir_exp_CONG_WEAK_def, SUBSET_REFL]
-);
+QED
 
-val bir_exp_CONG_WEAK_REFL = store_thm ("bir_exp_CONG_WEAK_REFL",
-  ``!e. bir_exp_CONG_WEAK e e``,
-SIMP_TAC std_ss [bir_exp_CONG_WEAK_def, SUBSET_REFL]);
+Theorem bir_exp_CONG_WEAK_REFL:
+  !e. bir_exp_CONG_WEAK e e
+Proof
+SIMP_TAC std_ss [bir_exp_CONG_WEAK_def, SUBSET_REFL]
+QED
 
 
-val bir_exp_CONG_WEAK_TRANS = store_thm ("bir_exp_CONG_WEAK_TRANS",
-  ``!e1 e2 e3. bir_exp_CONG_WEAK e1 e2 ==> bir_exp_CONG_WEAK e2 e3 ==> bir_exp_CONG_WEAK e1 e3``,
+Theorem bir_exp_CONG_WEAK_TRANS:
+  !e1 e2 e3. bir_exp_CONG_WEAK e1 e2 ==> bir_exp_CONG_WEAK e2 e3 ==> bir_exp_CONG_WEAK e1 e3
+Proof
 SIMP_TAC std_ss [bir_exp_CONG_WEAK_def, SUBSET_DEF,
-  bir_env_oldTheory.bir_env_vars_are_initialised_def] >>
-rpt strip_tac >>
-first_x_assum irule >>
-rpt strip_tac >- (
-  metis_tac[]
-) >- (
-  metis_tac[]
-) >- (
-  irule bir_env_oldTheory.bir_ext_env_exts_are_valid_SUBSET >>
-  metis_tac[SUBSET_DEF]
-));
+  bir_env_oldTheory.bir_env_vars_are_initialised_def]
+QED
 
 
-val bir_exp_CONG_WEAK_IS_CONG_SUBST = store_thm ("bir_exp_CONG_WEAK_IS_CONG_SUBST",
-``!v ve ve' e. bir_exp_CONG_WEAK ve ve' ==>
-               bir_exp_CONG_WEAK (bir_exp_subst1 v ve e) (bir_exp_subst1 v ve' e)``,
-
+Theorem bir_exp_CONG_WEAK_IS_CONG_SUBST:
+  !v ve ve' e. bir_exp_CONG_WEAK ve ve' ==>
+               bir_exp_CONG_WEAK (bir_exp_subst1 v ve e) (bir_exp_subst1 v ve' e)
+Proof
 REPEAT GEN_TAC >>
 Tactical.REVERSE (Cases_on `v IN bir_vars_of_exp e`) >- (
   ASM_SIMP_TAC std_ss [bir_exp_subst1_UNUSED_VAR, bir_exp_CONG_WEAK_REFL]
@@ -332,28 +276,22 @@ STRIP_TAC >>
   FULL_SIMP_TAC (std_ss++pred_setSimps.PRED_SET_ss) [SUBSET_DEF, bir_exp_subst1_USED_VARS] >>
   METIS_TAC[]
 ) >>
-`bir_exts_of_exp (bir_exp_subst1 v ve' e) SUBSET
- bir_exts_of_exp (bir_exp_subst1 v ve e)` by (
-  FULL_SIMP_TAC (std_ss++pred_setSimps.PRED_SET_ss) [SUBSET_DEF, bir_exp_subst1_USED_EXTS] >>
-  METIS_TAC[]
-) >>
 ASM_SIMP_TAC std_ss [bir_exp_subst1_TYPE_EQ_GEN] >>
 REPEAT STRIP_TAC >>
-`bir_eval_exp ve env ext_st = bir_eval_exp ve' env ext_st` suffices_by
+`bir_eval_exp ve env = bir_eval_exp ve' env` suffices_by
     METIS_TAC[bir_exp_subst1_EVAL_EQ_GEN] >>
 `?ty'. type_of_bir_exp ve = SOME ty'` by METIS_TAC[bir_exp_subst1_NO_TYPE_SOME] >>
 FULL_SIMP_TAC std_ss [] >>
-`(bir_vars_of_exp ve) SUBSET bir_vars_of_exp (bir_exp_subst1 v ve e) /\
- (bir_exts_of_exp ve) SUBSET bir_exts_of_exp (bir_exp_subst1 v ve e)` suffices_by (
-  METIS_TAC[bir_env_oldTheory.bir_env_vars_are_initialised_SUBSET,
-            bir_env_oldTheory.bir_ext_env_exts_are_valid_SUBSET]) >>
-ASM_SIMP_TAC std_ss [bir_exp_subst1_USED_VARS, bir_exp_subst1_USED_EXTS, SUBSET_UNION]
-);
+`(bir_vars_of_exp ve) SUBSET bir_vars_of_exp (bir_exp_subst1 v ve e)` suffices_by (
+  METIS_TAC[bir_env_oldTheory.bir_env_vars_are_initialised_SUBSET]) >>
+ASM_SIMP_TAC std_ss [bir_exp_subst1_USED_VARS, SUBSET_UNION]
+QED
 
 
-(* For practical purposed more insteresting is however a form that can be used
+(* For practical purposes more interesting is however a form that can be used
    as congruence rules. *)
-val bir_exp_CONG_WEAK_BASIC_CONG_RULES = store_thm ("bir_exp_CONG_WEAK_BASIC_CONG_RULES", ``
+Theorem bir_exp_CONG_WEAK_BASIC_CONG_RULES:
+  
 (!e e' ty ct.
       bir_exp_CONG_WEAK e e' ==>
       bir_exp_CONG_WEAK (BExp_Cast ct e ty) (BExp_Cast ct e' ty))
@@ -401,44 +339,45 @@ val bir_exp_CONG_WEAK_BASIC_CONG_RULES = store_thm ("bir_exp_CONG_WEAK_BASIC_CON
       bir_exp_CONG_WEAK a_e a_e' ==>
       bir_exp_CONG_WEAK v_e v_e' ==>
       bir_exp_CONG_WEAK (BExp_Store mem_e a_e en v_e) (BExp_Store mem_e' a_e' en v_e'))
-``,
 
-SIMP_TAC std_ss [bir_exp_CONG_WEAK_def, bir_vars_of_exp_def, bir_exts_of_exp_def,
+Proof
+SIMP_TAC std_ss [bir_exp_CONG_WEAK_def, bir_vars_of_exp_def,
   type_of_bir_exp_EQ_SOME_REWRS, bir_eval_exp_def,
   bir_env_oldTheory.bir_env_vars_are_initialised_UNION,
-  bir_env_oldTheory.bir_ext_env_exts_are_valid_UNION, SUBSET_DEF, IN_UNION,
+  SUBSET_DEF, IN_UNION,
   DISJ_IMP_THM, type_of_bir_exp_def] >>
-METIS_TAC[]);
+METIS_TAC[]
+QED
 
 
+Theorem bir_exp_CONG_WEAK_simp_IDEMPOTENT_AND:
+  !e. (?ty. bir_type_is_Imm ty /\ (type_of_bir_exp e = SOME ty)) ==>
+      bir_exp_CONG_WEAK (BExp_BinExp BIExp_And e e) e
+Proof
+METIS_TAC[bir_exp_CONG_simp_IDEMPOTENT_AND, bir_exp_CONG_WEAK_IS_WEAK]
+QED
 
 
-
-val bir_exp_CONG_WEAK_simp_IDEMPOTENT_AND = store_thm ("bir_exp_CONG_WEAK_simp_IDEMPOTENT_AND",
-``!e. (?ty. bir_type_is_Imm ty /\ (type_of_bir_exp e = SOME ty)) ==>
-      bir_exp_CONG_WEAK (BExp_BinExp BIExp_And e e) e``,
-METIS_TAC[bir_exp_CONG_simp_IDEMPOTENT_AND, bir_exp_CONG_WEAK_IS_WEAK]);
-
-
-val bir_exp_CONG_WEAK_simp_IDEMPOTENT_OR = store_thm ("bir_exp_CONG_WEAK_simp_IDEMPOTENT_OR",
-``!e. (?ty. bir_type_is_Imm ty /\ (type_of_bir_exp e = SOME ty)) ==>
-      bir_exp_CONG_WEAK (BExp_BinExp BIExp_Or e e) e``,
-METIS_TAC[bir_exp_CONG_simp_IDEMPOTENT_OR, bir_exp_CONG_WEAK_IS_WEAK]);
+Theorem bir_exp_CONG_WEAK_simp_IDEMPOTENT_OR:
+  !e. (?ty. bir_type_is_Imm ty /\ (type_of_bir_exp e = SOME ty)) ==>
+      bir_exp_CONG_WEAK (BExp_BinExp BIExp_Or e e) e
+Proof
+METIS_TAC[bir_exp_CONG_simp_IDEMPOTENT_OR, bir_exp_CONG_WEAK_IS_WEAK]
+QED
 
 
-val bir_exp_CONG_WEAK_simp_IF_THEN_ELSE_TF_EQ = store_thm ("bir_exp_CONG_WEAK_simp_IF_THEN_ELSE_TF_EQ",
-``!c e. (type_of_bir_exp c = SOME BType_Bool) ==>
-        bir_exp_CONG_WEAK (BExp_IfThenElse c e e) e``,
-
-SIMP_TAC std_ss [bir_exp_CONG_WEAK_def, bir_vars_of_exp_def, bir_exts_of_exp_def,
+Theorem bir_exp_CONG_WEAK_simp_IF_THEN_ELSE_TF_EQ:
+  !c e. (type_of_bir_exp c = SOME BType_Bool) ==>
+        bir_exp_CONG_WEAK (BExp_IfThenElse c e e) e
+Proof
+SIMP_TAC std_ss [bir_exp_CONG_WEAK_def, bir_vars_of_exp_def,
   type_of_bir_exp_def, SUBSET_DEF, IN_UNION,
-  bir_env_oldTheory.bir_ext_env_exts_are_valid_UNION, 
   bir_env_oldTheory.bir_env_vars_are_initialised_UNION, bir_eval_exp_def,
   pairTheory.pair_case_thm] >>
 REPEAT STRIP_TAC >- (
-  Cases_on `type_of_bir_exp e` >> fs[BType_Bool_def, bir_exts_of_exp_def]
+  Cases_on `type_of_bir_exp e` >> fs[BType_Bool_def]
 ) >>
-Cases_on `bir_eval_exp c env ext_st` >- (
+Cases_on `bir_eval_exp c env` >- (
   IMP_RES_TAC type_of_bir_exp_THM_with_init_vars >>
   FULL_SIMP_TAC (std_ss++holBACore_ss) []
 ) >>
@@ -447,13 +386,13 @@ subgoal `BType_Bool = type_of_bir_val x` >- (
   `x = va` by FULL_SIMP_TAC (std_ss++holBACore_ss) [] >>
   FULL_SIMP_TAC (std_ss++holBACore_ss) []
 ) >>
-Cases_on `bir_eval_exp e env ext_st` >- (
+Cases_on `bir_eval_exp e env` >- (
   FULL_SIMP_TAC (std_ss++holBACore_ss) []
 ) >>
 Cases_on `x` >> (
   FULL_SIMP_TAC (std_ss++holBACore_ss) [bir_eval_ifthenelse_def, BType_Bool_def]
 )
-);
+QED
 
 
 (* TODO: ADD MANY MORE! *)
