src/theory/bir/bir_programScript.sml
@@ -22,7 +22,7 @@ val _ = Datatype `bir_label_t =
 
 val _ = Datatype `bir_label_exp_t =
     BLE_Label bir_label_t
-  | BLE_Exp ('ext_state_t bir_exp_t)
+  | BLE_Exp bir_exp_t
 `;
 
 val _ = Datatype `bir_memop_t =
@@ -35,47 +35,43 @@ val _ = Datatype `bir_memop_t =
   Assign variable expression
   Assert expression
   Assume expression
-  ExtPut externName expression
 *)
 Datatype:
   bir_stmt_basic_t =
-  | BStmt_Assign bir_var_t ('ext_state_t bir_exp_t)
-  | BStmt_Assert ('ext_state_t bir_exp_t)
-  | BStmt_Assume ('ext_state_t bir_exp_t)
-(*  | BStmt_ExtPut string bir_exp_t (* string should be looked up as a (bir_val_t -> 'ext_state_t -> 'ext_state_t option) *) *)
+  | BStmt_Assign bir_var_t bir_exp_t
+  | BStmt_Assert bir_exp_t
+  | BStmt_Assume bir_exp_t
 End
 
 Datatype:
   bmc_stmt_basic_t =
   (* reg, address, cast, xcl, acq rel *)
-  | BMCStmt_Load bir_var_t ('ext_state_t bir_exp_t) ((bir_cast_t # bir_immtype_t) option) bool bool bool
+  | BMCStmt_Load bir_var_t bir_exp_t ((bir_cast_t # bir_immtype_t) option) bool bool bool
   (* success reg, address, value, xcl, acq, rel *)
-  | BMCStmt_Store bir_var_t ('ext_state_t bir_exp_t) ('ext_state_t bir_exp_t) bool bool bool
+  | BMCStmt_Store bir_var_t bir_exp_t bir_exp_t bool bool bool
   (* success reg, address, value, acq, rel *)
-  | BMCStmt_Amo bir_var_t ('ext_state_t bir_exp_t) ('ext_state_t bir_exp_t) bool bool
-  | BMCStmt_Assign bir_var_t ('ext_state_t bir_exp_t)
+  | BMCStmt_Amo bir_var_t bir_exp_t bir_exp_t bool bool
+  | BMCStmt_Assign bir_var_t bir_exp_t
   | BMCStmt_Fence bir_memop_t bir_memop_t
-  (* TODO: Should take view of the input *)
-(*  | BMCStmt_ExtPut string ('ext_state_t bir_exp_t) *)
-  | BMCStmt_Assert ('ext_state_t bir_exp_t)
-  | BMCStmt_Assume ('ext_state_t bir_exp_t)
+  | BMCStmt_Assert bir_exp_t
+  | BMCStmt_Assume bir_exp_t
 End
 
 Datatype:
   bir_stmt_end_t =
-  | BStmt_Jmp     ('ext_state_t bir_label_exp_t)
-  | BStmt_CJmp    ('ext_state_t bir_exp_t) ('ext_state_t bir_label_exp_t) ('ext_state_t bir_label_exp_t)
-  | BStmt_Halt    ('ext_state_t bir_exp_t)
+  | BStmt_Jmp     bir_label_exp_t
+  | BStmt_CJmp    bir_exp_t bir_label_exp_t bir_label_exp_t
+  | BStmt_Halt    bir_exp_t
 End
 
 Datatype:
   bir_generic_stmt_t =
   | BStmtB 'a
-  | BStmtE ('ext_state_t bir_stmt_end_t)
+  | BStmtE bir_stmt_end_t
 End
 
-Type bir_stmt_t = ``:('ext_state_t bir_stmt_basic_t,'ext_state_t) bir_generic_stmt_t``
-Type bmc_stmt_t = ``:('ext_state_t bmc_stmt_basic_t,'ext_state_t) bir_generic_stmt_t``
+Type bir_stmt_t = ``:bir_stmt_basic_t bir_generic_stmt_t``
+Type bmc_stmt_t = ``:bmc_stmt_basic_t bir_generic_stmt_t``
 
 val _ = Datatype `bir_mc_tags_t = <|
   mc_acq            : bool;
@@ -124,45 +120,44 @@ Datatype:
 |>
 End
 
-(* The extern block relation has three components on the RHS:
+(* The extern block relation has two components on the RHS:
  * The local BIR state (bir_state_t)
- * A polymorphic shared state ('shared_state_t)
- * an external state ('ext_state_t).
+ * and a polymorphic shared state ('shared_state_t).
  * Note that the shared state is not on the LHS, meaning
  * effectively that it is hard-coded as read-only.
  * For multicore BIR, the shared state contains the
  * set of other threads' local states and the shared memory. *)
 (* TODO: If this relation also has the BIR program on LHS, we can model block-relative jumps (i.e. "next block") *)
 Type beb_relation_t =
-  ``: (bir_state_t # 'shared_state_t # 'ext_state_t)
-    -> (bir_state_t # 'ext_state_t) -> bool``
+  ``: (bir_state_t # 'shared_state_t)
+    -> (bir_state_t) -> bool``
 
 val _ = Datatype `bir_generic_stmt_block_t = <|
   bb_label          : bir_label_t;
   bb_mc_tags        : bir_mc_tags_t option;
   bb_statements     : 'a list;
-  bb_last_statement : 'ext_state_t bir_stmt_end_t |>`;
+  bb_last_statement : bir_stmt_end_t |>`;
 
 val _ = Datatype `bir_ext_block_t = <|
   beb_label     : bir_label_t;
-  beb_relation  : ('ext_state_t, 'shared_state_t) beb_relation_t |>`;
+  beb_relation  : 'shared_state_t beb_relation_t |>`;
 
 val _ = Datatype `bir_generic_block_t =
-  | BBlock_Stmts (('a,'ext_state_t)  bir_generic_stmt_block_t)
-  | BBlock_Ext (('ext_state_t, 'shared_state_t) bir_ext_block_t)`;
+  | BBlock_Stmts ('a  bir_generic_stmt_block_t)
+  | BBlock_Ext ('shared_state_t bir_ext_block_t)`;
 
 Datatype:
-  bir_generic_program_t = BirProgram ((('a, 'ext_state_t, 'shared_state_t) bir_generic_block_t) list)
+  bir_generic_program_t = BirProgram ((('a, 'shared_state_t) bir_generic_block_t) list)
 End
 
-Type bir_stmt_block_t = `` :('ext_state_t bir_stmt_basic_t, 'ext_state_t) bir_generic_stmt_block_t``
-Type bmc_stmt_block_t = `` :('ext_state_t bmc_stmt_basic_t, 'ext_state_t) bir_generic_stmt_block_t``
+Type bir_stmt_block_t = `` :bir_stmt_basic_t bir_generic_stmt_block_t``
+Type bmc_stmt_block_t = `` :bmc_stmt_basic_t bir_generic_stmt_block_t``
 
-Type bir_block_t = `` :('ext_state_t bir_stmt_basic_t, 'ext_state_t, 'shared_state_t) bir_generic_block_t``
-Type bmc_block_t = `` :('ext_state_t bmc_stmt_basic_t, 'ext_state_t, 'shared_state_t) bir_generic_block_t``
+Type bir_block_t = `` :(bir_stmt_basic_t, 'shared_state_t) bir_generic_block_t``
+Type bmc_block_t = `` :(bmc_stmt_basic_t, 'shared_state_t) bir_generic_block_t``
 
-Type bir_program_t = ``:('ext_state_t bir_stmt_basic_t, 'ext_state_t, 'shared_state_t) bir_generic_program_t``
-Type bmc_program_t = ``:('ext_state_t bmc_stmt_basic_t, 'ext_state_t, 'shared_state_t) bir_generic_program_t``
+Type bir_program_t = ``:(bir_stmt_basic_t, 'shared_state_t) bir_generic_program_t``
+Type bmc_program_t = ``:(bmc_stmt_basic_t, 'shared_state_t) bir_generic_program_t``
 
 val bir_state_t_component_equality = DB.fetch "-" "bir_state_t_component_equality";
 val bir_programcounter_t_component_equality = DB.fetch "-" "bir_programcounter_t_component_equality";
@@ -172,9 +167,9 @@ TODO
 val bir_state_ss = rewrites (type_rws ``:bir_state_t``);
 val bir_status_ss = rewrites (type_rws ``:bir_status_t``);
 
-val bir_stmt_ss = rewrites ((type_rws ``:'ext_state_t bir_stmt_t``)
-                    @ (type_rws ``:'ext_state_t bir_stmt_end_t``)
-                    @ (type_rws ``:'ext_state_t bir_stmt_basic_t``));
+val bir_stmt_ss = rewrites ((type_rws ``:bir_stmt_t``)
+                    @ (type_rws ``:bir_stmt_end_t``)
+                    @ (type_rws ``:bir_stmt_basic_t``));
 *)
 
 (* ------------------------------------------------------------------------- *)
@@ -240,8 +235,8 @@ Cases_on `bir_get_program_block_info_by_label (BirProgram p) l` >| [
 
 Datatype:
   bir_generic_stmt_kind_t =
-    | BSGen (('a,'ext_state_t) bir_generic_stmt_t)
-    | BSExt (('ext_state_t,'shared_state_t) beb_relation_t)
+    | BSGen ('a bir_generic_stmt_t)
+    | BSExt ('shared_state_t beb_relation_t)
 End
 
 val bir_get_current_statement_def = Define `bir_get_current_statement p pc =
@@ -297,8 +292,8 @@ val bir_state_set_failed_def = Define `bir_state_set_failed st =
 (* ------------------------------------------------------------------------- *)
 
 Definition bir_exec_stmt_assign_def:
-  bir_exec_stmt_assign v ex (st:bir_state_t, ext_st:'ext_state_t) =
-   case bir_eval_exp ex st.bst_environ ext_st of
+  bir_exec_stmt_assign v ex st:bir_state_t =
+   case bir_eval_exp ex st.bst_environ of
      | SOME va => (case bir_env_write v va st.bst_environ of
                      | SOME env => (st with bst_environ := env)
                      | NONE => bir_state_set_typeerror st
@@ -307,66 +302,40 @@ Definition bir_exec_stmt_assign_def:
 End
 
 Definition bir_exec_stmt_assert_def:
-  bir_exec_stmt_assert ex (st:bir_state_t, ext_st :'ext_state_t) =
-  case (option_CASE (bir_eval_exp ex st.bst_environ ext_st) NONE bir_dest_bool_val) of
+  bir_exec_stmt_assert ex st:bir_state_t =
+  case (option_CASE (bir_eval_exp ex st.bst_environ) NONE bir_dest_bool_val) of
     | SOME T => st
     | SOME F => (st with bst_status := BST_AssertionViolated)
     | NONE => bir_state_set_typeerror st
 End
 
 Definition bir_exec_stmt_assume_def:
-  bir_exec_stmt_assume ex (st:bir_state_t, ext_st : 'ext_state_t) =
-  case (option_CASE (bir_eval_exp ex st.bst_environ ext_st) NONE bir_dest_bool_val) of
+  bir_exec_stmt_assume ex st:bir_state_t =
+  case (option_CASE (bir_eval_exp ex st.bst_environ) NONE bir_dest_bool_val) of
     | SOME T => st
     | SOME F => (st with bst_status := BST_AssumptionViolated)
     | NONE => bir_state_set_typeerror st
 End
 
-(*
-val bir_exec_stmt_ext_put_def = Define `bir_exec_stmt_ext_put (ext_name:string) ex (st:bir_state_t, ext_st:'ext_state_t) =
-  case bir_eval_exp ex st.bst_environ ext_st of
-    | SOME va =>
-     (case bir_lookup_put ext_name of
-      | SOME f =>
-       (case f va ext_st of
-         | SOME ext_st' => (st, ext_st')
-         | NONE => (bir_state_set_typeerror st, ext_st)
-       )
-      | NONE => (bir_state_set_typeerror st, ext_st)
-     )
-    | NONE => (bir_state_set_typeerror st, ext_st)`;
-*)
-
 val bir_exec_stmtB_def = Define `
-  (bir_exec_stmtB (BStmt_Assert ex) (st: bir_state_t, ext_st:'ext_state_t) = (bir_exec_stmt_assert ex (st, ext_st), ext_st)) /\
-  (bir_exec_stmtB (BStmt_Assume ex) (st, ext_st) = (bir_exec_stmt_assume ex (st, ext_st), ext_st)) /\
-  (bir_exec_stmtB (BStmt_Assign v ex) (st, ext_st) = (bir_exec_stmt_assign v ex (st, ext_st), ext_st)) (*/\
-  (bir_exec_stmtB (BStmt_ExtPut ext_name ex) (st, ext_st) = bir_exec_stmt_ext_put ext_name ex (st, ext_st))*)`;
+  (bir_exec_stmtB (BStmt_Assert ex) st:bir_state_t = bir_exec_stmt_assert ex st) /\
+  (bir_exec_stmtB (BStmt_Assume ex) st = bir_exec_stmt_assume ex st) /\
+  (bir_exec_stmtB (BStmt_Assign v ex) st = bir_exec_stmt_assign v ex st)`;
 
 val bir_exec_stmtB_exists =
   store_thm("bir_exec_stmtB_exists",
-  ``!h st ext_st:'ext_state_t.
-      ?st' ext_st'.
-        bir_exec_stmtB h (st, ext_st) = (st', ext_st')``,
+  ``!h st .
+      ?st'.
+        bir_exec_stmtB h st = st'``,
 
 Cases_on `h` >> (
   rpt strip_tac >>
   fs [bir_exec_stmtB_def]
-)(* >>
-fs [bir_exec_stmt_ext_put_def] >>
-Cases_on `bir_eval_exp b st.bst_environ ext_st` >> (
-  fs []
-) >>
-Cases_on `bir_lookup_put s` >> (
-  fs []
-) >>
-Cases_on `x' x ext_st` >> (
-  fs []
-) *)
+)
 );
 
-val bir_exec_stmt_halt_def = Define `bir_exec_stmt_halt ex (st:bir_state_t, ext_st:'ext_state_t) =
-  case bir_eval_exp ex st.bst_environ ext_st of
+val bir_exec_stmt_halt_def = Define `bir_exec_stmt_halt ex st:bir_state_t =
+  case bir_eval_exp ex st.bst_environ of
     | NONE => bir_state_set_typeerror st
     | SOME v => st with bst_status := BST_Halted v`;
 
@@ -376,52 +345,52 @@ val bir_exec_stmt_jmp_to_label_def = Define `bir_exec_stmt_jmp_to_label p l st =
     else (st with bst_status := (BST_JumpOutside l))`;
 
 val bir_eval_label_exp_def = Define `
-   (bir_eval_label_exp (BLE_Label l) env (ext_st:'ext_state_t) = SOME l) /\
-   (bir_eval_label_exp (BLE_Exp e) env ext_st = case bir_eval_exp e env ext_st of
+   (bir_eval_label_exp (BLE_Label l) env = SOME l) /\
+   (bir_eval_label_exp (BLE_Exp e) env = case bir_eval_exp e env of
       | SOME (BVal_Imm i) => SOME (BL_Address i)
       | _ => NONE
    )`;
 
-val bir_exec_stmt_jmp_def = Define `bir_exec_stmt_jmp p le (st, ext_st:'ext_state_t) =
-    case bir_eval_label_exp le st.bst_environ ext_st of
+val bir_exec_stmt_jmp_def = Define `bir_exec_stmt_jmp p le st =
+    case bir_eval_label_exp le st.bst_environ of
       | NONE => bir_state_set_typeerror st
       | SOME l => bir_exec_stmt_jmp_to_label p l st`;
 
-val bir_exec_stmt_cjmp_def = Define `bir_exec_stmt_cjmp p ec l1 l2 (st, ext_st:'ext_state_t) =
+val bir_exec_stmt_cjmp_def = Define `bir_exec_stmt_cjmp p ec l1 l2 st =
   let
-    vobc = option_CASE (bir_eval_exp ec st.bst_environ ext_st) NONE bir_dest_bool_val
+    vobc = option_CASE (bir_eval_exp ec st.bst_environ) NONE bir_dest_bool_val
   in
   case vobc of
-    | SOME T => bir_exec_stmt_jmp p l1 (st, ext_st)
-    | SOME F => bir_exec_stmt_jmp p l2 (st, ext_st)
+    | SOME T => bir_exec_stmt_jmp p l1 st
+    | SOME F => bir_exec_stmt_jmp p l2 st
     | NONE => bir_state_set_typeerror st`;
 
 
 val bir_exec_stmtE_def = Define `
-  (bir_exec_stmtE p (BStmt_Jmp l) (st, ext_st:'ext_state_t) = bir_exec_stmt_jmp p l (st, ext_st)) /\
-  (bir_exec_stmtE p (BStmt_CJmp e l1 l2) (st, ext_st) = bir_exec_stmt_cjmp p e l1 l2 (st, ext_st)) /\
-  (bir_exec_stmtE p (BStmt_Halt ex) (st, ext_st) = bir_exec_stmt_halt ex (st, ext_st))`;
+  (bir_exec_stmtE p (BStmt_Jmp l) st = bir_exec_stmt_jmp p l st) /\
+  (bir_exec_stmtE p (BStmt_CJmp e l1 l2) st = bir_exec_stmt_cjmp p e l1 l2 st) /\
+  (bir_exec_stmtE p (BStmt_Halt ex) st = bir_exec_stmt_halt ex st)`;
 
 
 val bir_exec_stmt_def = Define `
-  (bir_exec_stmt p (BStmtB (bst:'ext_state_t bir_stmt_basic_t)) (st:bir_state_t, ext_st:'ext_state_t) =
-     let (st', ext_st') = bir_exec_stmtB bst (st, ext_st) in
-     if bir_state_is_terminated st' then (st', ext_st') else (st' with bst_pc updated_by bir_pc_next, ext_st')) /\
-  (bir_exec_stmt p (BStmtE bst) (st, ext_st) = (bir_exec_stmtE p bst (st, ext_st), ext_st))`;
+  (bir_exec_stmt p (BStmtB bst) st:bir_state_t =
+     let st' = bir_exec_stmtB bst st in
+     if bir_state_is_terminated st' then st' else (st' with bst_pc updated_by bir_pc_next)) /\
+  (bir_exec_stmt p (BStmtE bst) st = bir_exec_stmtE p bst st)`;
 
 (* bmc_exec_block_ext is defined later, in the promising semantics *)
 Definition bir_exec_block_ext_def:
-  bir_exec_block_ext ext_fun (st:bir_state_t, ext_st:'ext_state_t) =
-    (CHOICE (ext_fun (st, EMPTY:bir_state_t -> bool, ext_st))):(bir_state_t # 'ext_state_t)
+  bir_exec_block_ext ext_fun st:bir_state_t =
+    (CHOICE (ext_fun (st, EMPTY:bir_state_t -> bool))):bir_state_t
 End
 
 Definition bir_exec_step_def:
-  bir_exec_step p (state : bir_state_t, ext_st:'ext_state_t) =
-  if (bir_state_is_terminated state) then (state, ext_st) else
+  bir_exec_step p (state : bir_state_t) =
+  if (bir_state_is_terminated state) then state else
     case (bir_get_current_statement p state.bst_pc) of
-    | NONE => (bir_state_set_failed state, ext_st)
-    | SOME $ BSGen stm => bir_exec_stmt p stm (state, ext_st)
-    | SOME $ BSExt rel => bir_exec_block_ext rel (state, ext_st)
+    | NONE => bir_state_set_failed state
+    | SOME $ BSGen stm => bir_exec_stmt p stm state
+    | SOME $ BSExt rel => bir_exec_block_ext rel state
 End
 
 
@@ -439,21 +408,21 @@ End
 (******************************)
 
 val bir_exec_infinite_steps_fun_def = Define `
-  (bir_exec_infinite_steps_fun p (st, ext_st:'ext_state_t) n = FUNPOW (bir_exec_step p) n (st,ext_st))`;
+  (bir_exec_infinite_steps_fun p st n = FUNPOW (bir_exec_step p) n st)`;
 
 
 val bir_exec_infinite_steps_fun_REWRS = store_thm ("bir_exec_infinite_steps_fun_REWRS",
-``(!p st ext_st. (bir_exec_infinite_steps_fun p (st, ext_st:'ext_state_t) 0 = (st, ext_st))) /\
-  (!p st ext_st n. (bir_exec_infinite_steps_fun p (st, ext_st:'ext_state_t) (SUC n) =
-     (bir_exec_infinite_steps_fun p (bir_exec_step p (st, ext_st)) n)))``,
+``(!p st. (bir_exec_infinite_steps_fun p st 0 = st)) /\
+  (!p st n. (bir_exec_infinite_steps_fun p st (SUC n) =
+     (bir_exec_infinite_steps_fun p (bir_exec_step p st) n)))``,
 
 SIMP_TAC std_ss [bir_exec_infinite_steps_fun_def, arithmeticTheory.FUNPOW] >>
 rpt strip_tac >>
-Cases_on `(bir_exec_step p (st,ext_st))` >>
+Cases_on `(bir_exec_step p st)` >>
 fs[bir_exec_infinite_steps_fun_def]);
 
 
-val bir_state_COUNT_PC_def = Define `bir_state_COUNT_PC (count_failing:bool, pc_cond) (st, ext_st:'ext_state_t) =
+val bir_state_COUNT_PC_def = Define `bir_state_COUNT_PC (count_failing:bool, pc_cond) st =
   case st.bst_status of
     | BST_JumpOutside l => pc_cond (bir_block_pc l)
     | BST_Running => pc_cond st.bst_pc
@@ -463,19 +432,19 @@ val bir_state_COUNT_PC_def = Define `bir_state_COUNT_PC (count_failing:bool, pc_
 
 (* How often was a PC with a certain property reached. *)
 val bir_exec_infinite_steps_fun_COUNT_PCs_def = Define
-  `(bir_exec_infinite_steps_fun_COUNT_PCs pc_cond p (st, ext_st:'ext_state_t) 0 = 0) /\
-   (bir_exec_infinite_steps_fun_COUNT_PCs pc_cond p (st, ext_st) (SUC n) =
+  `(bir_exec_infinite_steps_fun_COUNT_PCs pc_cond p st 0 = 0) /\
+   (bir_exec_infinite_steps_fun_COUNT_PCs pc_cond p st (SUC n) =
     let r = bir_exec_infinite_steps_fun_COUNT_PCs pc_cond p
-               (bir_exec_step p (st, ext_st)) n in
-    if (bir_state_COUNT_PC pc_cond (bir_exec_step p (st, ext_st))) then SUC r else r)`
+               (bir_exec_step p st) n in
+    if (bir_state_COUNT_PC pc_cond (bir_exec_step p st)) then SUC r else r)`
 
 
 
 (* After how many steps do we terminate ? *)
 val bir_exec_infinite_steps_COUNT_STEPS_def = Define `
-  bir_exec_infinite_steps_COUNT_STEPS pc_cond max_steps_opt p (st, ext_st:'ext_state_t) = (OLEAST i.
-     bir_state_is_terminated $ FST (bir_exec_infinite_steps_fun p (st, ext_st) i) \/
-     (max_steps_opt = SOME (bir_exec_infinite_steps_fun_COUNT_PCs pc_cond p (st, ext_st) i))
+  bir_exec_infinite_steps_COUNT_STEPS pc_cond max_steps_opt p st = (OLEAST i.
+     bir_state_is_terminated (bir_exec_infinite_steps_fun p st i) \/
+     (max_steps_opt = SOME (bir_exec_infinite_steps_fun_COUNT_PCs pc_cond p st i))
 )`;
 
 
@@ -488,14 +457,14 @@ val _ = Datatype `bir_execution_result_t =
        that the execution ended after "step_count" steps in state "st". During
        execution "pc_count" pcs that satisfy the given predicate where encountered
        (counting the pc of the final state st, but not the one of the initial state). *)
-    BER_Ended   num num (bir_state_t # 'ext_state_t)
+    BER_Ended   num num bir_state_t
 
     (* The execution does not terminate. Since the programs are finite, this means
        it loops. Therefore there are no step counts and no final state. *)
   | BER_Looping
 `;
 
-val bir_execution_result_ss = rewrites (type_rws ``:'ext_state_t bir_execution_result_t``);
+val bir_execution_result_ss = rewrites (type_rws ``:bir_execution_result_t``);
 
 val IS_BER_Ended_def = Define `
    (IS_BER_Ended (BER_Ended _ _ _) = T) /\
@@ -503,55 +472,55 @@ val IS_BER_Ended_def = Define `
 
 
 val IS_BER_Ended_EXISTS = store_thm ("IS_BER_Ended_EXISTS",
-``!ber. IS_BER_Ended ber <=> (?step_count pc_count final_st final_ext_st:'ext_state_t.
-        ber = BER_Ended step_count pc_count (final_st, final_ext_st))``,
+``!ber. IS_BER_Ended ber <=> (?step_count pc_count final_st.
+        ber = BER_Ended step_count pc_count final_st)``,
 
 Cases_on `ber`
->- (Cases_on `p` >> SIMP_TAC (std_ss++bir_execution_result_ss) [IS_BER_Ended_def])
+>- (SIMP_TAC (std_ss++bir_execution_result_ss) [IS_BER_Ended_def])
 >> SIMP_TAC (std_ss++bir_execution_result_ss) [IS_BER_Ended_def]);
 
 
-val valOf_BER_Ended_def = Define `valOf_BER_Ended (BER_Ended step_count pc_count (final_st, final_ext_st:'ext_state_t)) =
-  (step_count, pc_count, (final_st, final_ext_st))`;
+val valOf_BER_Ended_def = Define `valOf_BER_Ended (BER_Ended step_count pc_count final_st) =
+  (step_count, pc_count, final_st)`;
 
-val valOf_BER_Ended_steps_def = Define `valOf_BER_Ended_steps (BER_Ended step_count pc_count (final_st, final_ext_st:'ext_state_t)) =
-  (step_count, (final_st, final_ext_st))`;
+val valOf_BER_Ended_steps_def = Define `valOf_BER_Ended_steps (BER_Ended step_count pc_count final_st) =
+  (step_count, final_st)`;
 
 
 (* Now real execution. This is a clear definition, which is not well suited for evalation
    though. More efficient versions are derived later. We compute the no of steps and
    then execute this number of steps, recomputing values multiple times. *)
-val bir_exec_steps_GEN_def = Define `bir_exec_steps_GEN pc_cond p (state, ext_st:'ext_state_t) max_steps_opt =
-  let step_no = bir_exec_infinite_steps_COUNT_STEPS pc_cond max_steps_opt p (state, ext_st) in
+val bir_exec_steps_GEN_def = Define `bir_exec_steps_GEN pc_cond p state max_steps_opt =
+  let step_no = bir_exec_infinite_steps_COUNT_STEPS pc_cond max_steps_opt p state in
   (case step_no of
     | NONE => BER_Looping
     | SOME i => BER_Ended i
-                (bir_exec_infinite_steps_fun_COUNT_PCs pc_cond p (state, ext_st) i)
-                (bir_exec_infinite_steps_fun p (state, ext_st) i))`;
+                (bir_exec_infinite_steps_fun_COUNT_PCs pc_cond p state i)
+                (bir_exec_infinite_steps_fun p state i))`;
 
 
 (* A simple instance that just runs till termination. *)
 val bir_exec_steps_def = Define `
-  (bir_exec_steps p (state, ext_st:'ext_state_t) = bir_exec_steps_GEN (T, (\_. T)) p (state, ext_st) NONE)`;
+  (bir_exec_steps p state = bir_exec_steps_GEN (T, (\_. T)) p state NONE)`;
 
 (* A simple instance that counts all steps and has a fixed no of steps given.
    We are sure it terminates, therefore, the result is converted to a tuple. *)
 val bir_exec_step_n_def = Define `
-  bir_exec_step_n p (state, ext_st:'ext_state_t) n =
-  valOf_BER_Ended_steps (bir_exec_steps_GEN (T, (\_. T)) p (state, ext_st) (SOME n))`
+  bir_exec_step_n p state n =
+  valOf_BER_Ended_steps (bir_exec_steps_GEN (T, (\_. T)) p state (SOME n))`
 
 (* We might be interested in executing a certain no of blocks. *)
 val bir_exec_block_n_def = Define `
-  bir_exec_block_n p (state, ext_st:'ext_state_t) n =
-  valOf_BER_Ended (bir_exec_steps_GEN (F, (\pc. pc.bpc_index = 0)) p (state, ext_st) (SOME n))`
+  bir_exec_block_n p state n =
+  valOf_BER_Ended (bir_exec_steps_GEN (F, (\pc. pc.bpc_index = 0)) p state (SOME n))`
 
 (* Executing till a certain set of labels is useful as well. Since we might loop
    outside this set of labels, infinite runs are possible. *)
 val bir_exec_to_labels_n_def = Define `
-  bir_exec_to_labels_n ls p (state, ext_st:'ext_state_t) n =
-  bir_exec_steps_GEN (F, \pc. (pc.bpc_index = 0) /\ (pc.bpc_label IN ls)) p (state, ext_st) (SOME n)`
+  bir_exec_to_labels_n ls p state n =
+  bir_exec_steps_GEN (F, \pc. (pc.bpc_index = 0) /\ (pc.bpc_label IN ls)) p state (SOME n)`
 
 val bir_exec_to_labels_def = Define `
-  bir_exec_to_labels ls p (state, ext_st:'ext_state_t) = bir_exec_to_labels_n ls p (state, ext_st) 1`
+  bir_exec_to_labels ls p state = bir_exec_to_labels_n ls p state 1`
 
 val _ = export_theory();
