src/theory/bir-support/bir_extScript.sml
@@ -1,0 +1,29 @@
+open HolKernel Parse boolLib bossLib;
+
+open bir_program_valid_stateTheory;
+
+val _ = new_theory "bir_ext";
+
+
+(* This definition captures what an extern block must obey to play
+ * nice with the existing theorems in bir-support.
+ * Note this notion is stated with respect to a specific program *)
+(* TODO: Rename *)
+Definition well_formed_ext_def:
+  well_formed_ext p ext =
+    (bir_is_well_typed_ext ext /\
+    !st st'.
+    bir_exec_block_ext ext.beb_relation st = st' ==>
+    bir_is_valid_pc p st.bst_pc ==>
+    bir_is_valid_pc p st'.bst_pc)
+End
+
+(* The entire program is well-formed with respect to extern blocks *)
+Definition well_formed_prog_ext_def:
+  well_formed_prog_ext p =
+    !st ext.
+    bir_get_current_block p st.bst_pc = SOME (BBlock_Ext ext) ==>
+    well_formed_ext p ext
+End
+
+val _ = export_theory();
